src/fresh/CompCert/lib/FreeMonad.v
@@ -1,1 +1,1 @@
-../../../lib/FM/FreeMonad.v
+../../../lib/FM/FreeMonadB.v
